Remove parameters, fix broken semantics, initial attempt at defining heaps

src/semantics.lean
@@ -4,9 +4,20 @@ import syntax data.finsupp data.fintype
 
 universe u
 
-open signature nat list pexp
+open signature nat list
 
-/- Fix a signature. We treat object identities transparently. Each object identity is associated to a single class name. Given a finite set of object identities, there can always be a fresh object identity not in that set (thanks to Johannes Hölzl). Allocation of a fresh object results in an object with the same class name as allocated. Equality is decidable for objects. -/
+/- Fix a signature. We consider an interpretation of reference types and data types. Reference types are interpreted as object identities. Each object identity is associated to a single class name. Given a finite set of object identities, there can always be a fresh object identity not in that set (thanks to Johannes Hölzl). Allocation of a fresh object results in an object with the same class name as allocated. Equality is decidable for objects. Each record name is uniquely associated to a data type. A data type comprises an inhabited Lean type with decidable equality. The built-in boolean is associated to Lean's bool with false as default. -/
+structure datatype :=
+  (host : Type)
+  (inhabited_host: inhabited host)
+  (decidable_host: decidable_eq host)
+instance datatype.decidable_eq (d : datatype) :
+  decidable_eq d.host := d.decidable_host
+instance datatype.inhabited_eq (d : datatype) :
+  inhabited d.host := d.inhabited_host
+def datatype.default (d : datatype) : d.host :=
+  default d.host
+
 class objects (α β : Type) extends signature α :=
 (alloc: finset β → class_name α → β)
 (class_of: β → class_name α)
@@ -15,33 +26,45 @@ class objects (α β : Type) extends signature α :=
   (alloc x c) ∉ x)
 (alloc_class_of (x : finset β) (c : class_name α):
   class_of (alloc x c) = c)
+(data_type: record_name α → datatype)
+(data_type_boolean:
+  (data_type (boolean_name α)).host = bool)
+(data_type_boolean_inhabited:
+  (cast data_type_boolean (data_type (boolean_name α))
+    .inhabited_host.default) = ff)
 open objects
 
 variables {α β : Type} [objects α β]
 variable {c : class_name α}
 
-instance objects.decidable : decidable_eq β :=
+lemma data_type_booleanr [objects α β] :
+  bool = (data_type (boolean_name α)).host :=
+begin symmetry, apply data_type_boolean end
+instance objects.decidable_eq : decidable_eq β :=
   decidable_object α β
 
-/- We treat values as being of a type. A value of a reference type is an object of the same class, or null. A value of a data type is a term of the type in the host language. -/
+/- We treat values as being of a type. A value of a reference type is an object of the same class, or null. A value of a data type is a term of the associated type in Lean. -/
 @[derive decidable_eq]
 inductive value [objects α β] : type α → Type 1
 | object {c : class_name α} :
     {o : β // c = class_of α o} → value (type.ref c)
-| null (c : class_name α) : value (type.ref c)
-| term {r : record_name α} : data_Type r → value (type.data r)
+| null (c : class_name α) :
+    value (type.ref c)
+| term {r : record_name α} :
+    (data_type r).host → value (type.data r)
+/- The default value of a reference type is null, and the default value of a data type is the default in Lean. -/
 instance value.inhabited [objects α β] :
     Π{ty : type α}, inhabited (value ty)
 | (type.ref c) := ⟨value.null c⟩
-| (type.data r) := ⟨value.term (data_default r)⟩
+| (type.data r) := ⟨value.term (data_type r).default⟩
 -- Projection of value to term
 def value.unterm [objects α β] {r : record_name α} :
-    Π (x : value (type.data r)), data_Type r
+    Π (x : value (type.data r)), (data_type r).host
 | (value.term t) := t
 -- Projection of boolean value to bool
 def value.unbool [objects α β] :
   Π (x : value (boolean α)), bool
-| (value.term t) := cast (eq.symm data_Type_eq_bool) t
+| (value.term t) := cast (data_type_boolean α β) t
 -- Projection of value to potential object
 def value.unobject {c : class_name α} :
     Π (x : value (type.ref c)), option β
@@ -75,13 +98,6 @@ def value.elim_object {γ : Sort u} {c : class_name α}
   | (value.null .(c)), h := g h
   end
 
-/- For method m, we have a argument space Σ(m) consisting of an assignment of method parameters to values. -/
-@[derive decidable_eq]
-structure arg_space [objects α β]
-    {self : class_name α} (m : method_name self) :=
-  (map (p : param_name m) : value (param_type p))
-notation Σ(m) := arg_space m
-
 /- Given a list of types, we have a value list of values with matching types. -/
 @[derive decidable_eq]
 inductive vallist [objects α β] : list (type α) → Type 1
@@ -95,20 +111,43 @@ def vallist.default [objects α β] :
     (vallist.default l)
 instance vallist.inhabited [objects α β] (l : list (type α)) :
   inhabited (vallist l) := ⟨vallist.default l⟩
+/- A value list of a single type is just a value. -/
+def vallist.single [objects α β] {ty : type α}
+    (v : value ty) : vallist [ty] :=
+  vallist.cons v vallist.nil
+/- There is a unique value of a single value list. -/
+def vallist.the [objects α β] {ty : type α} :
+    vallist [ty] → value ty
+| (vallist.cons h vallist.nil) := h
+/- A value list of a single type can be appended at the front to form a new value list. -/
+def vallist.consl [objects α β]
+    {ty : type α} {l : list (type α)}
+    (h : vallist [ty]) (t : vallist l) : vallist (ty :: l) :=
+  vallist.cons (h.the) t
 /- Given a value list and an index in the list of types, we obtain a value. -/
 def vallist.lookup [objects α β] {ty : type α} :
     Π {l : context α}, vallist l → list_at ty l → value ty
 | (x :: xs) (vallist.cons v _) (list_at.here .(x) .(xs)) := v
 | (x :: xs) (vallist.cons _ ys) (list_at.tail .(x) zs) :=
     vallist.lookup ys zs
-/- Given a value list and an index and a new value, we obtain a new value list which updates the given index. -/
-def vallist.update [objects α β] {ty : type α} :
-    Π {l : context α}, vallist l → list_at ty l →
-    value ty → vallist l
-| (x :: xs) (vallist.cons _ tl) (list_at.here .(x) .(xs)) v :=
-    vallist.cons v tl
-| (x :: xs) (vallist.cons v ys) (list_at.tail .(x) zs) w :=
-    vallist.cons v (vallist.update ys zs w)
+
+/- For class C we have a state space Σ(C) consisting of a this identity and an assignment of fields to values. -/
+@[derive decidable_eq]
+structure state_space [objects α β] (self : class_name α) :=
+  (map (f : field_name self) : value (field_type f))
+  (this : value (type.ref self))
+  (N : value.not_null this)
+def state_space.id [objects α β] {self : class_name α}
+  (σ : state_space self) : β := value.the_object σ.this σ.N
+lemma state_space.class_of_id [objects α β]
+  {self : class_name α} (σ : state_space self) :
+  class_of α σ.id = self :=
+begin
+  unfold state_space.id, apply value.class_of_the_object
+end
+notation Σ(C) := state_space C
+
+/- A heap is a finite set of state spaces. TODO -/
 
 /- An event is either an asynchronous method call of some caller object to a callee object, its method, and for each parameter an argument value. Or, an event is a method selection. -/
 @[derive decidable_eq]
@@ -116,11 +155,11 @@ structure callsite (α β : Type) [objects α β] :=
   {c : class_name α}
   (o : {o : β // c = class_of α o})
   (m : method_name c)
-  (τ : Σ(m))
+  (τ : vallist (param_types m))
 def callsite.elim {γ : Sort u}
     (cs : callsite α β) (f : Π{c : class_name α}
       (o : {o : β // c = class_of α o})
-      (m : method_name c) (τ : Σ(m)),
+      (m : method_name c) (τ : vallist (param_types m)),
       cs = @callsite.mk α β _ c o m τ → γ) : γ :=
   match cs, rfl : (∀ b, cs = b → γ) with
   | ⟨o,m,τ⟩, h := f o m τ h
@@ -136,7 +175,8 @@ def event.to_callsite : event α β → callsite α β
 def event.o (e : event α β) : β := e.to_callsite.o
 def event.c (e : event α β) : class_name α := e.to_callsite.c
 def event.m (e : event α β) : method_name e.c := e.to_callsite.m
-def event.τ (e : event α β) : Σ(e.m) := e.to_callsite.τ
+def event.τ (e : event α β) : vallist (param_types e.m) :=
+  e.to_callsite.τ
 instance event.event_to_callsite : has_coe (event α β)
   (callsite α β) := ⟨event.to_callsite⟩
 
@@ -234,53 +274,44 @@ def global_history.fresh (θ : global_history α β)
 /- An active process consists of: an argument space (of the current method), a value list (of the local variables), and a list of statements. -/
 variables {C : class_name α} {e : tenv C}
 structure active_process (e : tenv C) :=
-  (args : Σ(e.current)) (store : vallist e.locals)
+  (args : vallist e.args) (store : vallist e.locals)
   (body : list (statement e))
-/- For class C we have a state space Σ(C) consisting of a this identity and an assignment of fields to values. -/
-@[derive decidable_eq]
-structure state_space [objects α β] (self : class_name α) :=
-  (map (f : field_name self) : value (field_type f))
-  (this : value (type.ref self))
-  (N : value.not_null this)
-def state_space.id [objects α β] {self : class_name α}
-  (σ : state_space self) : β := value.the_object σ.this σ.N
-lemma state_space.class_of_id [objects α β]
-  {self : class_name α} (σ : state_space self) :
-  class_of α σ.id = self :=
-begin
-  unfold state_space.id, apply value.class_of_the_object
-end
-/- A state space can be updated. -/
-def state_space.update (f : field_name C)
-    (v : value (field_type f)) : state_space C → state_space C
-| ⟨map, this, N⟩ := ⟨λg, if H : f = g
-    then cast begin rewrite H end v else map g,this,N⟩
-notation Σ(C) := state_space C
 
 /- Given an object space and active process, we can lookup the value of a read variable. -/
 def active_process.lookup (σ : Σ(C)) (π : active_process e)
     {tx : type α} : rvar e tx → value tx
 | (rvar.tvar t) := cast begin rewrite t.H, refl end σ.this
 | (rvar.fvar f) := cast begin rewrite f.H end $ σ.map f.idx
-| (rvar.pvar p) := cast begin rewrite p.H end $ π.args.map p.idx
+| (rvar.pvar p) := π.args.lookup p.idx
 | (rvar.lvar l) := π.store.lookup l.idx
-/- Evaluating a pure expression, Val(p)(σ,π). -/
+/- Evaluating a pure expression to a list of values. -/
 def eval (σ : Σ(C)) (π : active_process e) :
-    Π {ty : type α}, pexp e ty → value ty
-| bool (requal l r) := value.term $
-    cast data_Type_eq_bool $ to_bool (eval l = eval r)
-| _ (lookup r) := π.lookup σ r
-| _ (const _ v) := value.term v
-| _ (app f r) := value.term $ f (eval r).unterm
-/- Evaluating an argument list to an argument space. -/
-def evallist (σ : Σ(C)) (π : active_process e)
-    {c : class_name α} {m : method_name c} : arglist e m → Σ(m)
-| ⟨map⟩ := ⟨λa, eval σ π (map a)⟩
+    Π {l : list (type α)}, pexp e l → vallist l
+| _ (pexp.requal l r) := vallist.single $ value.term $
+    cast data_type_booleanr $ to_bool (eval l = eval r)
+| _ (pexp.lookup r) := vallist.single (π.lookup σ r)
+| _ (pexp.const .(e) s) := _
+| _ (pexp.app f r) := _
+| _ (pexp.cons h t) := vallist.consl (eval h) (eval t)
 
+/- A state space can be updated. -/
+def state_space.update
+    (f : field_name C) (v : value (field_type f)) :
+    state_space C → state_space C
+| ⟨map, this, N⟩ := ⟨λg, if H : f = g
+    then cast begin rewrite H end v else map g,this,N⟩
 /- A state space can be updated, given a field variable in a typing environment related to the same class. -/
 def state_space.updatev {ty : type α}
     (fvar : fvar e ty) (v : value ty) (σ : Σ(C)) : Σ(C) :=
   σ.update fvar.idx (cast begin rewrite fvar.H end v)
+/- Given a value list and an index and a new value, we obtain a new value list which updates the given index. -/
+def vallist.update [objects α β] {ty : type α} :
+    Π {l : context α}, vallist l → list_at ty l →
+    value ty → vallist l
+| (x :: xs) (vallist.cons _ tl) (list_at.here .(x) .(xs)) v :=
+    vallist.cons v tl
+| (x :: xs) (vallist.cons v ys) (list_at.tail .(x) zs) w :=
+    vallist.cons v (vallist.update ys zs w)
 
 /- We fix a program, and global history. -/
 variables (p : program α) (θ : global_history α β)
@@ -290,13 +321,11 @@ inductive process {α : Type} [objects α β] (C : class_name α)
 | active (env : tenv C) (a : active_process env) : process
 /- Given a method and arguments, we can activate a process. -/
 def process.activate (C : class_name α) (m : method_name C)
-    (τ : Σ(m)) : process C :=
+    (τ : vallist (param_types m)) : process C :=
   process.active (p.body m).tenv ⟨τ,default _,(p.body m).S⟩
 /- A local configuration is an object and its process. -/
-structure local_config (α β : Type) [objects α β]
-  := (C : class_name α) (σ : Σ(C)) (m : process C)
-
-open stmt process svar rvar
+structure local_config (α β : Type) [objects α β] :=
+  (C : class_name α) (σ : Σ(C)) (m : process C)
 
 /- A local result is the result of taking a step at a local configuration. -/
 inductive local_result (α β : Type) [objects α β]
@@ -310,11 +339,11 @@ open local_result
 /- A step is taken on a local configuration. -/
 def local_config.step : local_config α β → local_result α β
 /- If the process is inactive, we obtain a pending method call. If no method call is pending, no step is taken. Otherwise, the next local configuration is an active process with the arguments of the selected method, a default store, and the body of the method as statement; additionally, a selection event is generated. -/
-| ⟨C, σ, nil .(C)⟩ := let e := θ.sched σ.id in
+| ⟨C, σ, process.nil _⟩ := let e := θ.sched σ.id in
     option.elim e
       (λ_, no_step α β)
       (λd h, callsite.elim d (λc o m τ g,
-      let p := activate p c m τ,
+      let p := process.activate p c m τ,
         G : process c = process C := begin
           have : (θ.sched σ.id) = some ⟨o, m, τ⟩,
             rw ← g, assumption,
@@ -330,41 +359,53 @@ def local_config.step : local_config α β → local_result α β
         end
       in external_step ⟨C, σ, cast G p⟩ (event.selection d)))
 /- Otherwise, there is an active process. We look at the list of statements. If the list is empty, the process becomes inactive. -/
-| ⟨C, σ, active _ ⟨τ,ℓ,nil⟩⟩ := internal_step ⟨C, σ, nil _⟩
+| ⟨C, σ, process.active _ ⟨τ,ℓ,nil⟩⟩ :=
+    internal_step ⟨C, σ, process.nil _⟩
 /- Otherwise, there is a current statement. If the current statement is an if statement, for which we evaluate the boolean pure expression. If it is true, we replace the current statement by those of the then-branch. Otherwise, we replace the current statement by those of the else-branch. -/
-| ⟨C, σ, active env π@⟨τ,ℓ,(ite p thenb elseb :: t)⟩⟩ :=
-    internal_step $ match (eval σ π p).unbool with
-    | tt := ⟨C, σ, active env ⟨τ,ℓ,to_list thenb ++ t⟩⟩
-    | ff := ⟨C, σ, active env ⟨τ,ℓ,to_list elseb ++ t⟩⟩
+| ⟨C, σ, process.active env
+      π@⟨τ,ℓ,(stmt.ite p thenb elseb :: t)⟩⟩ :=
+    internal_step $ match (eval σ π p).the.unbool with
+    | tt := ⟨C, σ, process.active env
+        ⟨τ,ℓ,stmt.to_list thenb ++ t⟩⟩
+    | ff := ⟨C, σ, process.active env
+        ⟨τ,ℓ,stmt.to_list elseb ++ t⟩⟩
     end
 /- Otherwise, there is a while statement. We evaluate the boolean pure expression. If it is true, we prepend the body to all statements, before but including the current while statement. Otherwise, we discard the current statement. -/
-| ⟨C, σ, active env π@⟨τ,ℓ,S@(while p dob :: t)⟩⟩ :=
-    internal_step $ match (eval σ π p).unbool with
-    | tt := ⟨C, σ, active env ⟨τ,ℓ,to_list dob ++ S⟩⟩
-    | ff := ⟨C, σ, active env ⟨τ,ℓ,t⟩⟩
+| ⟨C, σ, process.active env π@⟨τ,ℓ,S@(stmt.while p dob :: t)⟩⟩ :=
+    internal_step $ match (eval σ π p).the.unbool with
+    | tt := ⟨C, σ, process.active env
+        ⟨τ,ℓ,stmt.to_list dob ++ S⟩⟩
+    | ff := ⟨C, σ, process.active env ⟨τ,ℓ,t⟩⟩
     end
 /- Otherwise, we consider the assignment statement. We evaluate the pure expression, and the result is taken to update the variable on the left-hand side: if it is a field then the object space field state is updated, otherwise it is a local and the store is updated. In both cases, the current statement is discarded. -/
-| ⟨C, σ, active env π@⟨τ,ℓ,(assign (fvar f) p :: t)⟩⟩ :=
-    internal_step
-      ⟨C, σ.updatev f (eval σ π p), active env ⟨τ,ℓ,t⟩⟩
-| ⟨C, σ, active env π@⟨τ,ℓ,(assign (lvar ⟨l⟩) p :: t)⟩⟩ :=
-    internal_step
-      ⟨C, σ, active env ⟨τ,ℓ.update l (eval σ π p),t⟩⟩
+| ⟨C, σ, process.active env
+      π@⟨τ,ℓ,(stmt.assign (svar.fvar f) p :: t)⟩⟩ :=
+    internal_step ⟨C, σ.updatev f (eval σ π p).the,
+      process.active env ⟨τ,ℓ,t⟩⟩
+| ⟨C, σ, process.active env
+      π@⟨τ,ℓ,(stmt.assign (svar.lvar ⟨l⟩) p :: t)⟩⟩ :=
+    internal_step ⟨C, σ, process.active env
+      ⟨τ,ℓ.update l (eval σ π p).the,t⟩⟩
 /- Otherwise, we have an async statement. We evaluate the argument list to a value list; the object pure expression is evaluated to an object value. If that value is null, no step is taken. Otherwise, we generate a method selection event with our object as caller and the appropriate call site, and discard the current statement. -/
-| ⟨C, σ, active env π@⟨τ,ℓ,(async c m G o τ' :: t)⟩⟩ :=
+| ⟨C, σ, process.active env
+      π@⟨τ,ℓ,(stmt.async c m G o τ' :: t)⟩⟩ :=
     (π.lookup σ o).elim_object
-      (λo h, external_step ⟨C, σ,active env ⟨τ,ℓ,t⟩⟩
-        (event.call σ.id ⟨o,m,evallist σ π τ'⟩))
+      (λo h, external_step ⟨C, σ, process.active env ⟨τ,ℓ,t⟩⟩
+        (event.call σ.id ⟨o,m,eval σ π τ'⟩))
       (λ_, crash α β)
 /- Otherwise, we have an alloc statement. We evaluate the argument list to a value list. A fresh object identity is obtained from the global history, and stored in the variable. A call event to the constructor of the freshly obtained object is generated with an approriate call site, and the current statement is discarded. -/
-| ⟨C, σ, active env π@⟨τ,ℓ,(alloc c (fvar f) τ' :: t)⟩⟩ :=
+| ⟨C, σ, process.active env
+      π@⟨τ,ℓ,(stmt.alloc c (svar.fvar f) τ' :: t)⟩⟩ :=
     let o := θ.fresh c, new := value.object o in
-      external_step ⟨C, σ.updatev f new, active env ⟨τ,ℓ,t⟩⟩
-        (event.call σ.id ⟨o,ctor c,evallist σ π τ'⟩)
-| ⟨C, σ, active env π@⟨τ,ℓ,(alloc c (lvar ⟨l⟩) τ' :: t)⟩⟩ :=
+      external_step ⟨C, σ.updatev f new,
+        process.active env ⟨τ,ℓ,t⟩⟩
+        (event.call σ.id ⟨o,ctor c,eval σ π τ'⟩)
+| ⟨C, σ, process.active env
+      π@⟨τ,ℓ,(stmt.alloc c (svar.lvar ⟨l⟩) τ' :: t)⟩⟩ :=
     let o := θ.fresh c, new := value.object o in
-      external_step ⟨C, σ, active env ⟨τ,ℓ.update l new,t⟩⟩
-        (event.call σ.id ⟨o,ctor c,evallist σ π τ'⟩)
+      external_step ⟨C, σ,
+        process.active env ⟨τ,ℓ.update l new,t⟩⟩
+        (event.call σ.id ⟨o,ctor c,eval σ π τ'⟩)
 
 /- A global configuration is a finite set of object configurations and a global history. -/
 @[derive decidable_eq]
